Engine: add abstract meta engine

Engine/Meta/Meta.v
@@ -24,8 +24,54 @@ Section Meta.
   Context {params: LindenParameters}.
   Context (rer: RegExpRecord).
 
-Definition meta_supported_regex (r:regex) : bool :=
-  is_pike_regex r.
+(* abstract heuristic for picking an anchored and anchored engine  *)
+Record meta_heuristic := {
+  meta_supported_regex : regex -> bool;
+  pick_anchored : regex -> input -> AnchoredEngine rer;
+  anchored_supported : forall r inp,
+    meta_supported_regex r = true ->
+    let engine := pick_anchored r inp in
+    engine.(supported_regex rer) r = true;
+  pick_unanchored : regex -> input -> UnanchoredEngine rer;
+  unanchored_supported : forall r inp,
+    meta_supported_regex r = true ->
+    let engine := pick_unanchored r inp in
+    engine.(un_supported_regex rer) r = true;
+}.
+
+(* entry point for looking for a match for a regex r in an input inp *)
+Definition meta_search {heuristic:meta_heuristic} (r:regex) (inp:input) : option leaf :=
+  match @try_lit_search _ rer BruteForceStrSearch r inp with
+  | Ok ol => ol
+  | Unsupported =>
+    match @try_anchored_search _ _ (heuristic.(pick_anchored) r inp) r inp with
+    | Ok ol => ol
+    | Unsupported => @un_exec _ _ (heuristic.(pick_unanchored) r inp) r inp
+    end
+  end.
+
+Theorem meta_search_correct {heuristic:meta_heuristic}:
+  forall r inp tree,
+    heuristic.(meta_supported_regex) r = true ->
+    is_tree rer [Areg (lazy_prefix r)] inp Groups.GroupMap.empty forward tree ->
+    first_leaf tree inp = @meta_search heuristic r inp.
+Proof.
+  intros r inp tree Hsup Htree.
+  unfold meta_search.
+  destruct try_lit_search as [|ol'] eqn:Hlit.
+  - (* literal search failed, try anchored search *)
+    destruct try_anchored_search as [|ol'] eqn:Hanch.
+    + (* anchored search not applicable, fall back to unanchored search *)
+      pose proof (heuristic.(unanchored_supported) r inp).
+      eauto using un_exec_correct.
+    + (* anchored search succeeded *)
+      pose proof (heuristic.(anchored_supported) r inp).
+      eapply try_anchored_search_correct in Hanch as <-; eauto.
+  - (* literal search succeeded *)
+    eapply try_lit_search_correct in Hlit; eauto.
+Qed.
+
+(** Specialized Meta engine with a custom heuristic *)
 
 (* The configuration of a Meta engine search *)
 Record meta_config := {
@@ -35,93 +81,71 @@ Record meta_config := {
   memory_limit : option nat;
 }.
 
-Definition memobt_peak_memory_usage (r:regex) (inp:input) : nat :=
-  regex_size r * total_length inp.
-
-(* an anchored search with heuristics *)
-Definition meta_search_anchored (config:meta_config) (r:regex) (inp:input) : option leaf :=
-  let can_use_memobt := match config.(memory_limit) with
-    | Some lim => memobt_peak_memory_usage r inp <=? lim
-    | None => true
-  end in
-  if can_use_memobt then
-    @exec _ _ (@MemoBTAnchoredEngine _ rer) r inp
-  else
-    @exec _ _ (@PikeVMAnchoredEngine VMSlist _ rer) r inp.
-
-Theorem meta_search_anchored_correct (config:meta_config):
-  forall r inp tree,
-    meta_supported_regex r = true ->
-    is_tree rer [Areg r] inp Groups.GroupMap.empty forward tree ->
-    first_leaf tree inp = meta_search_anchored config r inp.
-Proof.
-  intros r inp tree Hsup Htree.
-  unfold meta_search_anchored.
-  case_if.
-  - (* use the MemoBT engine *)
-    eauto using exec_correct.
-  - (* use the PikeVM engine *)
-    eauto using exec_correct.
-Qed.
-
-Instance MetaSearchAnchored (config:meta_config): AnchoredEngine rer := {
-  exec := meta_search_anchored config;
-  supported_regex := meta_supported_regex;
-  exec_correct := meta_search_anchored_correct config
-}.
-
 (* MemoBT supports lazy_prefix *)
 Lemma lazy_prefix_supported_memobt:
   @lazy_prefix_supported _ rer (MemoBTAnchoredEngine rer).
 Proof. intro r. eauto. Qed.
 
-Definition search (config:meta_config) (r:regex) (inp:input) : option leaf :=
-  match @try_lit_search _ rer BruteForceStrSearch r inp with
-  | Ok ol => ol
-  | Unsupported =>
-    match @try_anchored_search _ _ (@MetaSearchAnchored config) r inp with
-    | Ok ol => ol
-    | Unsupported =>
-        let can_use_memobt := match config.(memory_limit) with
-          | Some lim => memobt_peak_memory_usage r inp <=? lim
-          | None => true
-        end in
-        if can_use_memobt then
-          @un_exec _ _ (@SearchAccOnceEngine _ rer BruteForceStrSearch (@UnanchorEngine _ rer (@MemoBTAnchoredEngine _ rer) lazy_prefix_supported_memobt)) r inp
-        else
-          @un_exec _ _ (@SearchAccOnceEngine _ rer BruteForceStrSearch (@PikeVMUnanchoredEngine VMSlist _ rer BruteForceStrSearch)) r inp
-    end
+Definition memobt_peak_memory_usage (r:regex) (inp:input) : nat :=
+  regex_size r * total_length inp.
+
+Definition can_use_memobt (config:meta_config) (r:regex) (inp:input) : bool :=
+  match config.(memory_limit) with
+    | Some lim => memobt_peak_memory_usage r inp <=? lim
+    | None => true
   end.
 
+(* a choice of an anchored engine *)
+Definition pick_meta_anchored (config:meta_config) (r:regex) (inp:input) : AnchoredEngine rer :=
+  if can_use_memobt config r inp then
+    @MemoBTAnchoredEngine _ rer
+  else
+    @PikeVMAnchoredEngine VMSlist _ rer.
 
-Theorem search_correct (config:meta_config):
-  forall r inp tree,
-    meta_supported_regex r = true ->
-    is_tree rer [Areg (lazy_prefix r)] inp Groups.GroupMap.empty forward tree ->
-    first_leaf tree inp = search config r inp.
+(* a choice of an unanchored engine *)
+Definition pick_meta_unanchored (config:meta_config) (r:regex) (inp:input) : UnanchoredEngine rer :=
+  if can_use_memobt config r inp then
+    @SearchAccOnceEngine _ rer BruteForceStrSearch (@UnanchorEngine _ rer (@MemoBTAnchoredEngine _ rer) lazy_prefix_supported_memobt)
+  else
+    @SearchAccOnceEngine _ rer BruteForceStrSearch (@PikeVMUnanchoredEngine VMSlist _ rer BruteForceStrSearch).
+
+Lemma pick_meta_anchored_supported (config:meta_config):
+  forall r inp,
+    is_pike_regex r = true ->
+    let engine := pick_meta_anchored config r inp in
+    engine.(supported_regex rer) r = true.
 Proof.
-  intros r inp tree Hsup Htree.
-  unfold search.
-  unfold meta_supported_regex in Hsup.
-  destruct try_lit_search as [|ol'] eqn:Hlit.
-  - (* literal search failed, try anchored search *)
-    destruct try_anchored_search as [|ol'] eqn:Hanch.
-    + (* anchored search not applicable, fall back to unanchored search *)
-      case_if.
-      * (* use the MemoBT engine *)
-        eauto using un_exec_correct.
-      * (* use the PikeVM engine *)
-        eauto using un_exec_correct.
-    + (* anchored search succeeded *)
-      eapply try_anchored_search_correct in Hanch as <-; eauto.
-  - (* literal search succeeded *)
-    eapply try_lit_search_correct in Hlit; eauto.
+  unfold pick_meta_anchored.
+  intros.
+  destruct can_use_memobt; eauto.
 Qed.
 
+Lemma pick_meta_unanchored_supported (config:meta_config):
+  forall r inp,
+    is_pike_regex r = true ->
+    let engine := pick_meta_unanchored config r inp in
+    engine.(un_supported_regex rer) r = true.
+Proof.
+  unfold pick_meta_unanchored.
+  intros.
+  destruct can_use_memobt; eauto.
+Qed.
+
+(* A specialized search function that deploys all verified optimizations *)
+Definition search (config:meta_config) (r:regex) (inp:input) : option leaf :=
+  @meta_search {|
+    meta_supported_regex := is_pike_regex;
+    pick_anchored := pick_meta_anchored config;
+    anchored_supported := pick_meta_anchored_supported config;
+    pick_unanchored := pick_meta_unanchored config;
+    unanchored_supported := pick_meta_unanchored_supported config;
+  |} r inp.
+
+(* proof that the new search function is an anchored engine itself *)
 Instance MetaEngine (config:meta_config): UnanchoredEngine rer := {
   un_exec := search config;
-  un_supported_regex := meta_supported_regex;
-  un_exec_correct := search_correct config
+  un_supported_regex := is_pike_regex;
+  un_exec_correct := ltac:(intros; now apply meta_search_correct);
 }.
 
 End Meta.
